Finish all admitted proof of CPS.v

CloseLemmas.v
@@ -1,11 +1,8 @@
 Require Export SystemFR.Tactics.
 
-Require Export SystemFR.Syntax.
 Require Export SystemFR.SubstitutionLemmas.
-Require Export SystemFR.FVLemmas.
 Require Export SystemFR.FVLemmasLists.
-Require Export SystemFR.ListUtils.
-Require Export SystemFR.AssocList.
+Require Export SystemFR.TOpenTClose.
 
 Lemma close_nothing:
   forall x t k,
@@ -22,6 +19,17 @@ Lemma close_nothing2:
     close k t x = t.
 Proof.
   intros; apply close_nothing; repeat step || rewrite_any.
+Qed.
+
+Lemma open_close3:
+  forall t k1 k2 x rep,
+    fv rep = nil ->
+    wf rep 0 ->
+    k1 <> k2 ->
+    open k1 (close k2 t x) rep =
+    close k2 (open k1 t rep) x.
+Proof.
+  induction t; repeat step || t_equality || rewrite_any || rewrite close_nothing2 by auto.
 Qed.
 
 Lemma substitute_close:
@@ -59,4 +67,68 @@ Lemma substitute_tclose:
 Proof.
   induction t;
     repeat step || t_equality || t_lookup || rewrite tclose_nothing2 by (steps; eauto with fv).
+Qed.
+
+Fixpoint closes k T xs :=
+  match xs with
+  | nil => T
+  | x :: xs => close k (closes (S k) T xs) x
+  end.
+
+Lemma is_erased_term_close:
+  forall t k x,
+    is_erased_term t ->
+    is_erased_term (close k t x).
+Proof.
+  induction t; steps.
+Qed.
+
+Lemma is_erased_type_close:
+  forall T k x,
+    is_erased_type T ->
+    is_erased_type (close k T x).
+Proof.
+  induction T; steps; eauto using is_erased_term_close.
+Qed.
+
+#[global]
+Hint Resolve is_erased_term_close: erased.
+#[global]
+Hint Resolve is_erased_type_close: erased.
+
+Lemma is_erased_type_closes:
+  forall xs k T,
+    is_erased_type T ->
+    is_erased_type (closes k T xs).
+Proof.
+  induction xs; steps; eauto with erased.
+Qed.
+
+#[global]
+Hint Resolve is_erased_type_closes: erased.
+
+Lemma open_closes:
+  forall xs x T v i,
+    fv v = nil ->
+    wf v 0 ->
+    wf T 0 ->
+    open (length xs + i) (closes i T (xs ++ x :: nil)) v =
+    closes i (psubstitute T ((x, v) :: nil) term_var) xs.
+Proof.
+  induction xs; repeat step || rewrite open_close; eauto with wf.
+  rewrite open_close3; steps; eauto with lia.
+  rewrite <- PeanoNat.Nat.add_succ_r.
+  rewrite_any; steps.
+Qed.
+
+Lemma open_closes_zero:
+  forall xs x T v,
+    fv v = nil ->
+    wf v 0 ->
+    wf T 0 ->
+    open (length xs) (closes 0 T (xs ++ x :: nil)) v =
+    closes 0 (psubstitute T ((x, v) :: nil) term_var) xs.
+Proof.
+  intros.
+  rewrite <- (PeanoNat.Nat.add_0_r (length xs)); eauto using open_closes.
 Qed.
