WFLemmas.v
@@ -141,3 +141,10 @@ Proof.
 Qed.
 
 Hint Resolve wf_build_nat: wf.
+
+Lemma wf_fvar: forall x tag k, wf (fvar x tag) k.
+Proof.
+  repeat light.
+Qed.
+
+Hint Resolve wf_fvar : wf.
